Multiple minor changes.

examples/machine-code/lisp/lisp_proofScript.sml
@@ -1,8 +1,7 @@
 open HolKernel boolLib bossLib Parse; val _ = new_theory "lisp_proof";
 
 open stringTheory finite_mapTheory pred_setTheory listTheory sumTheory;
-open lisp_typeTheory lisp_semanticsTheory;
-open lisp_evalTheory;
+open lisp_typeTheory lisp_semanticsTheory lisp_evalTheory;
 
 val _ = numLib.prefer_num();
 
@@ -157,6 +156,7 @@ val (iR_ev_rules,iR_ev_ind,iR_ev_cases) =
     iR_ap (FunCon fc,args,a) (FunConSem fc args))
   /\
   (!fn el args s a.
+    ~(MEM (func2sexp fn) [Sym "quote"; Sym "cond"]) /\
     iR_evl (el,a) args /\ iR_ap (fn,args,a) s /\ (LENGTH args = LENGTH el)
     ==> iR_ev (App fn el,a) s)
   /\
@@ -173,6 +173,7 @@ val (iR_ev_rules,iR_ev_ind,iR_ev_cases) =
     iR_ev (Ite ((e1,e2)::el),a) s)
   /\
   (!x fn args s a.
+    ~(MEM (func2sexp fn) [Sym "quote"; Sym "cond"]) /\
     iR_ap (fn,args,iFunBind a x fn) s ==> iR_ap(Label x fn,args,a) s)
   /\
   (!fv args s a.
@@ -182,7 +183,9 @@ val (iR_ev_rules,iR_ev_ind,iR_ev_cases) =
     iR_ap (OUTR(LIST_LOOKUP fv a),args,a) s ==> iR_ap (FunVar fv,args,a) s)
   /\
   (!xl e args s a.
-    (LENGTH args = LENGTH xl) /\ iR_ev (e,iVarBind a xl args) s
+    (LENGTH args = LENGTH xl) /\ 
+    (!a2. (FILTER (\x. ~(MEM (FST x) xl)) a = FILTER (\x. ~(MEM (FST x) xl)) a2) ==> 
+          iR_ev (e,iVarBind a2 xl args) s)
     ==> iR_ap (Lambda xl e,args,a) s)
   /\
   (!a.
@@ -335,18 +338,19 @@ val repeat_cdr_1 = prove(
   THEN SIMP_TAC std_ss [LET_DEF,LISP_SUB_def,SExp_11]);
 
 val iVarBind_EXISTS = prove(
-  ``!a xl args. (LENGTH xl = LENGTH args) ==>
-                ?xs. (iVarBind a xl args = xs ++ a) /\ (LENGTH xs = LENGTH args)``,
-  Induct_on `xl`
-  THEN Cases_on `args` THEN SIMP_TAC std_ss [LENGTH,DECIDE ``~(SUC n = 0)``]
-  THEN REWRITE_TAC [iVarBind_def]
+  ``!a xl args. ?xs. (iVarBind a xl args = xs ++ a) /\ (LENGTH xs = LENGTH xl)``,
+  Induct_on `xl` THEN Cases_on `args` THEN REWRITE_TAC [iVarBind_def]
   THEN1 (STRIP_TAC THEN Q.EXISTS_TAC `[]` THEN SIMP_TAC std_ss [APPEND,LENGTH])
-  THEN REPEAT STRIP_TAC THEN RES_TAC
-  THEN Q.PAT_ASSUM `!a. ?xs. bbb` (STRIP_ASSUME_TAC o Q.SPEC `(h',INL h)::a`)
-  THEN ASM_SIMP_TAC std_ss []
-  THEN Q.EXISTS_TAC `xs ++ [(h',INL h)]`
-  THEN SIMP_TAC std_ss [APPEND,LENGTH_APPEND,LENGTH,GSYM APPEND_ASSOC]
-  THEN DECIDE_TAC);
+  THEN1 (STRIP_TAC THEN Q.EXISTS_TAC `[]` THEN SIMP_TAC std_ss [APPEND,LENGTH])
+  THEN REPEAT STRIP_TAC THEN1
+    (POP_ASSUM (STRIP_ASSUME_TAC o Q.SPECL [`(h,INL (A Nil))::a`,`[]`])
+     THEN Q.EXISTS_TAC `SNOC (h,INL (A Nil)) xs` 
+     THEN ASM_SIMP_TAC std_ss [LENGTH_SNOC,LENGTH]
+     THEN ASM_SIMP_TAC std_ss [SNOC_APPEND,GSYM APPEND_ASSOC,APPEND])
+  THEN POP_ASSUM (STRIP_ASSUME_TAC o Q.SPECL [`(h',INL h)::a`,`t`])
+     THEN Q.EXISTS_TAC `SNOC (h',INL h) xs` 
+     THEN ASM_SIMP_TAC std_ss [LENGTH_SNOC,LENGTH]
+     THEN ASM_SIMP_TAC std_ss [SNOC_APPEND,GSYM APPEND_ASSOC,APPEND]);
 
 val sexpression_IF = prove(
   ``!b. sexpression2sexp (if b then True else False) = LISP_TEST b``,
@@ -394,8 +398,129 @@ val lisp_mult_lemma = prove(
   THEN `!x. MEM x args ==> ?n. x = A (Number n)` by METIS_TAC []
   THEN RES_TAC THEN METIS_TAC []);
 
+val LISP_REDUCE_AUX_def = Define `
+  (LISP_REDUCE_AUX 0 xs alist = ((alist:(string # (sexpression + func)) list),Val 0)) /\
+  (LISP_REDUCE_AUX n xs [] = ([],Val n)) /\
+  (LISP_REDUCE_AUX (SUC n) xs ((y,z)::ys) = 
+    if MEM (Sym y) xs then LISP_REDUCE_AUX n xs ys
+                else ((y,z)::ys,Val (SUC n)))`;
+
+val LISP_REDUCE_A_def = Define `
+  LISP_REDUCE_A (stack,xs,alist) = 
+    if isDot stack /\ isVal (CAR stack) 
+    then FST (LISP_REDUCE_AUX (getVal (CAR stack)) xs alist) else alist`;
+
+val LISP_REDUCE_S_def = Define `
+  LISP_REDUCE_S (stack,xs,alist) = 
+    if isDot stack /\ isVal (CAR stack)  
+    then let s = (SND (LISP_REDUCE_AUX (getVal (CAR stack)) xs alist)) in
+      if s = Val 0 then CDR stack else Dot s (CDR stack)
+    else stack`;
+
+val lisp_find_in_list_thm = prove(
+  ``!xs x. 
+      ?exp2 x2 y2. 
+      (lisp_find_in_list (CAR (pair2sexp (q,r)),x,list2sexp xs,z,stack,alist,l) =
+         (exp2,x2,y2,z,stack,alist,l)) /\
+      ((exp2 = Sym "nil") = ~MEM (Sym q) xs)``,
+  Induct THEN ONCE_REWRITE_TAC [lisp_find_in_list_def]
+  THEN ASM_SIMP_TAC std_ss [MEM,list2sexp_def,isDot_def,CAR_def,CDR_def,LET_DEF]
+  THEN Cases_on `r` THEN FULL_SIMP_TAC std_ss [pair2sexp_def,CAR_def]
+  THEN REPEAT STRIP_TAC THEN Cases_on `Sym q = h` 
+  THEN ASM_SIMP_TAC std_ss [EVAL ``Sym "t" = Sym "nil"``]);
+
+val lisp_reduce_alist_aux_EQ = prove(
+  ``!xs alist exp x y.
+      ?exp2 x2 y2. 
+        lisp_reduce_alist_aux (exp,x,y,Val n,Dot (list2sexp xs) stack,alist2sexp alist,l) =
+          let (alist,z) = LISP_REDUCE_AUX n xs alist in
+            (exp2,x2,y2,z,Dot (list2sexp xs) stack,alist2sexp alist,l)``,
+  Induct_on `n` THEN Cases_on `alist` 
+  THEN SIMP_TAC std_ss [alist2sexp_def,list2sexp_def,MAP,LISP_REDUCE_AUX_def,LET_DEF]
+  THEN ONCE_REWRITE_TAC [lisp_reduce_alist_aux_def]
+  THEN SIMP_TAC std_ss [SExp_11,isDot_def,DECIDE ``~(SUC n = 0)``,CAR_def,CDR_def,LET_DEF]
+  THEN ASSUME_TAC (GEN_ALL lisp_find_in_list_thm) THEN REPEAT STRIP_TAC
+  THEN Cases_on `h` THEN helperLib.SEP_I_TAC "lisp_find_in_list"
+  THEN ASM_SIMP_TAC std_ss [LISP_REDUCE_AUX_def,LISP_SUB_def] THEN REPEAT STRIP_TAC
+  THEN Cases_on `MEM (Sym q) xs` THEN ASM_SIMP_TAC std_ss [GSYM alist2sexp_def,LET_DEF]
+  THEN FULL_SIMP_TAC std_ss [alist2sexp_def,MAP,list2sexp_def,CDR_def]
+  THEN helperLib.SEP_I_TAC "lisp_reduce_alist_aux"
+  THEN ASM_SIMP_TAC std_ss [LET_DEF] THEN METIS_TAC []);
+
+val lisp_reduce_alist_EQ = prove(
+  ``!stack exp xs x y z l alist.
+      ?x2 z2. 
+        lisp_reduce_alist (exp,x,Dot (list2sexp xs) y,z,stack,alist2sexp alist,l) = 
+         (exp,x2,Dot (list2sexp xs) y,z2, LISP_REDUCE_S (stack,xs,alist), 
+          alist2sexp (LISP_REDUCE_A (stack,xs,alist)),l)``,
+  STRIP_TAC
+  THEN `?n s x1 x2. (stack = Sym s) \/ (stack = Dot x1 x2) \/ (stack = Val n)` by
+         (Cases_on `stack` THEN ASM_SIMP_TAC std_ss [SExp_11,SExp_distinct] THEN METIS_TAC [])
+  THEN ASM_SIMP_TAC std_ss [lisp_reduce_alist_def,
+         LISP_REDUCE_A_def,LISP_REDUCE_S_def,isDot_def,LET_DEF,CAR_def,CDR_def]
+  THEN `?n1 s1 x3 x4. (x1 = Sym s1) \/ (x1 = Dot x3 x4) \/ (x1 = Val n1)` by
+         (Cases_on `x1` THEN ASM_SIMP_TAC std_ss [SExp_11,SExp_distinct] THEN METIS_TAC [])
+  THEN FULL_SIMP_TAC std_ss [isDot_def,isSym_def,isVal_def] 
+  THEN REPEAT STRIP_TAC
+  THEN STRIP_ASSUME_TAC (helperLib.MATCH_INST (SPEC_ALL lisp_reduce_alist_aux_EQ)
+         ``lisp_reduce_alist_aux
+       (Dot (list2sexp xs) (Dot (Dot exp x2) (Dot (list2sexp xs) y)),
+        Dot (Dot exp x2) (Dot (list2sexp xs) y),list2sexp xs,Val n1,
+        Dot (list2sexp xs) (Dot (Dot exp x2) (Dot (list2sexp xs) y)),
+        alist2sexp alist,l)``)
+  THEN ASM_SIMP_TAC std_ss [getVal_def,CDR_def,LET_DEF]  
+  THEN Cases_on `LISP_REDUCE_AUX n1 xs alist` THEN ASM_SIMP_TAC std_ss []
+  THEN REPEAT STRIP_TAC THEN Cases_on `r = Val 0` 
+  THEN ASM_SIMP_TAC std_ss [CAR_def,CDR_def]);
+
+val FILTER_LISP_REDUCE_A = prove(
+  ``!a stack xl.
+      FILTER (λx. ¬MEM (FST x) xl) (LISP_REDUCE_A (stack,MAP Sym xl,a)) = 
+      FILTER (λx. ¬MEM (FST x) xl) a``,
+  SIMP_TAC std_ss [LISP_REDUCE_A_def]
+  THEN Cases_on `stack` THEN ASM_SIMP_TAC std_ss [isDot_def,CAR_def]
+  THEN Cases_on `S'` THEN ASM_SIMP_TAC std_ss [isVal_def,CAR_def,getVal_def]
+  THEN Q.SPEC_TAC (`n`,`n`) THEN Induct_on `a` 
+  THEN Cases_on `n` THEN ASM_SIMP_TAC std_ss [FILTER,LISP_REDUCE_AUX_def]
+  THEN Cases THEN ASM_SIMP_TAC std_ss [FILTER,LISP_REDUCE_AUX_def,MEM_MAP,SExp_11]
+  THEN REPEAT STRIP_TAC THEN Cases_on `MEM q xl` THEN ASM_SIMP_TAC std_ss [FILTER]);
+
+val repeat_cdr_thm = prove(
+  ``!n exp y z stack a l.
+      (repeat_cdr (exp,Val n,y,z,stack,a,l) =
+                  (exp,Val 0,y,z,stack,FUNPOW CDR n a,l))``, 
+  Induct THEN ONCE_REWRITE_TAC [repeat_cdr_def]
+  THEN REWRITE_TAC [iVarBind_def,APPEND]
+  THEN SIMP_TAC std_ss [SExp_11,DECIDE ``~(SUC n = 0)``,LET_DEF,arithmeticTheory.FUNPOW]
+  THEN ASM_SIMP_TAC std_ss [LISP_SUB_def]);
+  
+val FUNPOW_CDR_iVarBind = prove(
+  ``!a xs ys. FUNPOW CDR (LENGTH xs) (alist2sexp (iVarBind a xs ys)) = alist2sexp a``,
+  REPEAT STRIP_TAC THEN STRIP_ASSUME_TAC (Q.SPECL [`a`,`xs`,`ys`] iVarBind_EXISTS)
+  THEN POP_ASSUM (ASSUME_TAC o GSYM) THEN ASM_SIMP_TAC std_ss []
+  THEN Q.SPEC_TAC (`xs'`,`ts`) THEN REPEAT (POP_ASSUM (K ALL_TAC))
+  THEN Induct THEN SIMP_TAC std_ss [arithmeticTheory.FUNPOW,LENGTH,APPEND] 
+  THEN Cases_on `h` THEN Cases_on `r`
+  THEN FULL_SIMP_TAC std_ss [MAP,pair2sexp_def,list2sexp_def,CDR_def,alist2sexp_def]);
+
+val LISP_REDUCE_AUX_IMP = prove(
+  ``!n a x alist m.
+      (LISP_REDUCE_AUX n x a = (alist,m)) ==> 
+      getVal m <= n /\ isVal m /\
+      (alist2sexp alist = FUNPOW CDR (n - getVal m) (alist2sexp a))``,
+  Induct THEN Cases_on `a`
+  THEN SIMP_TAC std_ss [LISP_REDUCE_AUX_def,getVal_def,arithmeticTheory.FUNPOW,isVal_def]
+  THEN Cases_on `h`    
+  THEN SIMP_TAC std_ss [LISP_REDUCE_AUX_def,getVal_def,arithmeticTheory.FUNPOW]
+  THEN REVERSE (Cases_on `MEM (Sym q) x`) 
+  THEN ASM_SIMP_TAC std_ss [getVal_def,arithmeticTheory.FUNPOW,isVal_def]
+  THEN REPEAT STRIP_TAC THEN RES_TAC THEN1 DECIDE_TAC
+  THEN `SUC n − getVal m = SUC (n - getVal m)` by DECIDE_TAC 
+  THEN ASM_SIMP_TAC std_ss [arithmeticTheory.FUNPOW]
+  THEN ASM_SIMP_TAC std_ss [alist2sexp_def,MAP,list2sexp_def,CDR_def]);
+ 
 val iR_ev_LEMMA = let
-  val th = (IndDefRules.derive_mono_strong_induction [] (iR_ev_rules,iR_ev_ind))
+  val th = iR_ev_ind
   val th = Q.SPECL [`lisp_eval_ok`,`lisp_func_ok`,
             `\(xl,a) yl. EVERY I (MAP (\(x,y). lisp_eval_ok (x,a) y) (ZIP (xl,yl)))`] th
   val th = SIMP_RULE std_ss [ZIP,MAP,EVERY_DEF] th
@@ -405,9 +530,6 @@ val iR_ev_LEMMA = let
     THEN CONV_TAC ((QUANT_CONV o QUANT_CONV) (RAND_CONV
            (REWRITE_CONV [GSYM lisp_eval_hide_def])))
     THEN ONCE_REWRITE_TAC [lisp_eval_def]
-(*
-set_goal([],goal)
-*)
   val th = (hd o CONJUNCTS o MP th o prove) (goal,
   STRIP_TAC THEN1
    (INIT_TAC
@@ -445,7 +567,7 @@ set_goal([],goal)
    (INIT_TAC
     THEN SIMP_TAC std_ss [LET_DEF,isSym_def,isDot_def,CDR_def,CAR_def]
     THEN ONCE_REWRITE_TAC [lisp_app_def]
-    THEN IMP_RES_TAC iR_ap_LEMMA
+(*    THEN IMP_RES_TAC iR_ap_LEMMA  *)
     THEN FULL_SIMP_TAC std_ss [MEM]
     THEN Cases_on `el = []` THEN1
      (FULL_SIMP_TAC std_ss [list2sexp_def,MAP,isDot_def,LET_DEF]
@@ -475,7 +597,7 @@ set_goal([],goal)
     THEN SIMP_TAC std_ss [False_def,sexpression2sexp_def,atom2sexp_def,
            lisp_eval_hide_def,LET_DEF,CAR_def]
     THEN POP_ASSUM MP_TAC
-    THEN POP_ASSUM (K ALL_TAC)
+  (*  THEN POP_ASSUM (K ALL_TAC) *)
     THEN POP_ASSUM (STRIP_ASSUME_TAC o Q.SPECL [`Dot (Sym "cond") stack`,`y`,`Dot
        (Dot (Dot (term2sexp e1) (Dot (term2sexp e2) (Sym "nil")))
           (list2sexp (MAP
@@ -498,7 +620,7 @@ set_goal([],goal)
     THEN SIMP_TAC std_ss [False_def,sexpression2sexp_def,atom2sexp_def,
            lisp_eval_hide_def,LET_DEF,CAR_def]
     THEN POP_ASSUM MP_TAC
-    THEN POP_ASSUM (K ALL_TAC)
+ (*   THEN POP_ASSUM (K ALL_TAC) *)
     THEN POP_ASSUM MP_TAC
     THEN POP_ASSUM (STRIP_ASSUME_TAC o Q.SPECL [`Dot (Sym "cond") stack`,`y`,`Dot
        (Dot (Dot (term2sexp e1) (Dot (term2sexp e2) (Sym "nil")))
@@ -569,6 +691,9 @@ set_goal([],goal)
     THEN ONCE_REWRITE_TAC [lisp_func_def]
     THEN SIMP_TAC std_ss [CAR_def,CDR_def,isDot_def,isSym_def,list2sexp_def,SExp_11]
     THEN FULL_SIMP_TAC std_ss [IN_INSERT,LET_DEF,CAR_def,CDR_def]
+    THEN ASSUME_TAC (GEN_ALL lisp_reduce_alist_EQ)
+    THEN helperLib.SEP_I_TAC "lisp_reduce_alist"
+    THEN ASM_SIMP_TAC std_ss []
     THEN STRIP_ASSUME_TAC (Q.SPEC `list2sexp (MAP sexpression2sexp args)` lisp_length_EQ)
     THEN ASM_SIMP_TAC std_ss []
     THEN SIMP_TAC std_ss [CAR_def,CDR_def,isDot_def,isSym_def,list2sexp_def,SExp_11]
@@ -576,20 +701,16 @@ set_goal([],goal)
     THEN REWRITE_TAC [alist2sexp_def,LISP_LENGTH_THM,LENGTH_MAP]
     THEN Q.PAT_ASSUM `LENGTH args = LENGTH xl` (ASSUME_TAC o GSYM)
     THEN SIMP_TAC std_ss [CAR_def,CDR_def,isDot_def,isSym_def,list2sexp_def,SExp_11]
-    THEN (STRIP_ASSUME_TAC o UNDISCH o REWRITE_RULE [LENGTH_MAP] o
-      Q.SPECL [`MAP Sym xl`,`MAP sexpression2sexp args`,
-        `MAP pair2sexp a`,`list2sexp (MAP Sym xl)`,
-        `Dot (Dot (term2sexp e) (Sym "nil"))
-             (Dot (Val (LENGTH (args: sexpression list))) stack)`,
-        `list2sexp (MAP pair2sexp a)`,`l`]) zip_yz_lemma
-    THEN ASM_SIMP_TAC std_ss [CAR_def,CDR_def]
+    THEN ASSUME_TAC (GEN_ALL zip_yz_lemma) THEN helperLib.SEP_I_TAC "zip_yz" 
+    THEN POP_ASSUM MP_TAC THEN ASM_SIMP_TAC std_ss [LENGTH_MAP]
+    THEN REPEAT STRIP_TAC THEN ASM_SIMP_TAC std_ss [CAR_def,CDR_def]
     THEN POP_ASSUM (K ALL_TAC)
-    THEN `list2sexp (REVERSE
+    THEN `!zs. list2sexp (REVERSE
           (MAP (\(x,y). Dot x y)
              (ZIP (MAP Sym xl,MAP sexpression2sexp args))) ++
-        MAP pair2sexp a) = alist2sexp (iVarBind a xl args)` by
+           MAP pair2sexp zs) = 
+          alist2sexp (iVarBind zs xl args)` by
      (Q.PAT_ASSUM `LENGTH xl = LENGTH args` MP_TAC
-      THEN Q.SPEC_TAC (`a`,`zs`)
       THEN Q.SPEC_TAC (`xl`,`xs`)
       THEN Q.SPEC_TAC (`args`,`ys`)
       THEN REPEAT (POP_ASSUM (K ALL_TAC))
@@ -603,35 +724,43 @@ set_goal([],goal)
     THEN POP_ASSUM MP_TAC
     THEN POP_ASSUM (K ALL_TAC)
     THEN STRIP_TAC
+    THEN Q.PAT_ASSUM `!a2.bbb` (ASSUME_TAC o 
+            Q.SPEC `LISP_REDUCE_A (stack,MAP Sym xl,a)`)
+    THEN FULL_SIMP_TAC std_ss [FILTER_LISP_REDUCE_A]
     THEN Q.PAT_ASSUM `!x.bbb` (STRIP_ASSUME_TAC o Q.SPECL
-          [`x'`,`list2sexp []`,`Dot (Val (LENGTH (args:sexpression list))) stack`,`l`])
-    THEN ASM_REWRITE_TAC []
+          [`x'`,`list2sexp []`,`Dot (Val (LENGTH (args:sexpression list))) 
+                                    (LISP_REDUCE_S (stack,MAP Sym xl,a))`,`l`])
+    THEN ASM_REWRITE_TAC [] THEN POP_ASSUM (K ALL_TAC)
     THEN ONCE_REWRITE_TAC [lisp_eval_def]
     THEN REWRITE_TAC [EVAL ``TASK_CONT = TASK_EVAL``]
     THEN REWRITE_TAC [EVAL ``TASK_CONT = TASK_FUNC``]
     THEN SIMP_TAC std_ss [SExp_distinct,lisp_cont_def,LET_DEF,isDot_def,CDR_def,CAR_def]
-    THEN `repeat_cdr
-          (sexpression2sexp s,Val (LENGTH args),y',TASK_CONT,stack,
-           alist2sexp (iVarBind a xl args),l) =
-       (sexpression2sexp s,Val 0,y',TASK_CONT,stack,
-           alist2sexp a,l)` by
-     (IMP_RES_TAC (Q.SPEC `a` iVarBind_EXISTS)
-      THEN POP_ASSUM (STRIP_ASSUME_TAC o SPEC_ALL)
-      THEN FULL_SIMP_TAC std_ss []
-      THEN Q.PAT_ASSUM `LENGTH xs = LENGTH args` MP_TAC
-      THEN Q.SPEC_TAC (`a`,`a`)
-      THEN Q.SPEC_TAC (`args`,`args`)
-      THEN Q.SPEC_TAC (`xs`,`xs`)
-      THEN REPEAT (POP_ASSUM (K ALL_TAC))
-      THEN Induct
-      THEN Cases_on `args` THEN SIMP_TAC std_ss [LENGTH,DECIDE ``~(SUC n = 0)``]
-      THEN ONCE_REWRITE_TAC [repeat_cdr_def]
-      THEN REWRITE_TAC [iVarBind_def,APPEND]
-      THEN SIMP_TAC std_ss [SExp_11,DECIDE ``~(SUC n = 0)``,LET_DEF]
-      THEN SIMP_TAC std_ss [LISP_SUB_def,alist2sexp_def]
-      THEN SIMP_TAC std_ss [MAP,pair2sexp_def,list2sexp_def,CDR_def]
-      THEN METIS_TAC [alist2sexp_def])
-    THEN ASM_SIMP_TAC std_ss [alist2sexp_def,lisp_eval_hide_def]
+    THEN SIMP_TAC std_ss [repeat_cdr_thm]
+    THEN POP_ASSUM (ASSUME_TAC o GSYM) THEN ASM_SIMP_TAC std_ss []
+    THEN ASM_SIMP_TAC std_ss [FUNPOW_CDR_iVarBind,GSYM alist2sexp_def]
+    THEN SIMP_TAC std_ss [LISP_REDUCE_S_def,LISP_REDUCE_A_def]
+    THEN REVERSE (Cases_on `isDot stack /\ isVal (CAR stack)`)
+    THEN1 (FULL_SIMP_TAC std_ss [lisp_eval_hide_def] THEN METIS_TAC [])
+    THEN FULL_SIMP_TAC std_ss []
+    THEN `?n s2. stack = Dot (Val n) s2` by METIS_TAC [isVal_thm,isDot_thm,CAR_def]
+    THEN FULL_SIMP_TAC std_ss [CAR_def,CDR_def,getVal_def]
+    THEN ONCE_REWRITE_TAC [ONCE_REWRITE_RULE [GSYM lisp_eval_hide_def] lisp_eval_def]
+    THEN REWRITE_TAC [EVAL ``TASK_CONT = TASK_EVAL``]
+    THEN REWRITE_TAC [EVAL ``TASK_CONT = TASK_FUNC``,isDot_def]
+    THEN SIMP_TAC std_ss [lisp_cont_def,LET_DEF,CAR_def,CDR_def,isDot_def,repeat_cdr_thm]  
+    THEN `?alist m. LISP_REDUCE_AUX n (MAP Sym xl) a = (alist,m)` by METIS_TAC [pairTheory.PAIR]    
+    THEN ASM_SIMP_TAC std_ss []
+    THEN IMP_RES_TAC LISP_REDUCE_AUX_IMP
+    THEN Cases_on `m = Val 0` THEN ASM_SIMP_TAC std_ss [getVal_def]    
+    THEN1 METIS_TAC [lisp_eval_hide_def]
+    THEN ONCE_REWRITE_TAC [lisp_eval_def]
+    THEN REWRITE_TAC [EVAL ``TASK_CONT = TASK_EVAL``]
+    THEN REWRITE_TAC [EVAL ``TASK_CONT = TASK_FUNC``,isDot_def]
+    THEN SIMP_TAC std_ss [lisp_cont_def,LET_DEF,CAR_def,CDR_def,isDot_def,repeat_cdr_thm]  
+    THEN `?i. m = Val i` by METIS_TAC [isVal_thm]
+    THEN FULL_SIMP_TAC std_ss [SExp_11,isDot_def,repeat_cdr_thm,getVal_def]
+    THEN `i + (n - i) = n` by DECIDE_TAC 
+    THEN FULL_SIMP_TAC std_ss [GSYM arithmeticTheory.FUNPOW_ADD,lisp_eval_hide_def]
     THEN METIS_TAC []))
   in th end;
 
@@ -703,6 +832,35 @@ val LIST_LOOKUP_fmap2list_list2fmap = prove(
   THEN REWRITE_TAC [list2fmap_def,LIST_LOOKUP_def]
   THEN ASM_SIMP_TAC std_ss [FAPPLY_FUPDATE_THM]);
 
+val FILTER_T = prove(
+  ``!xs. FILTER (\x. T) xs = xs``,
+  Induct THEN SRW_TAC [] []);
+
+val list2fmap_iVarBind = prove(
+  ``!xs ys zs. list2fmap (iVarBind xs ys zs) = VarBind (list2fmap xs) ys zs``,
+  Induct_on `ys` THEN SIMP_TAC std_ss [iVarBind_def,VarBind_def]
+  THEN Cases_on `zs` THEN ASM_SIMP_TAC std_ss [iVarBind_def,VarBind_def,list2fmap_def]);
+
+val VarBind_EQ = prove(
+  ``!xs ys f1 f2. 
+      (DRESTRICT f1 (COMPL (LIST_TO_SET xs)) = 
+       DRESTRICT f2 (COMPL (LIST_TO_SET xs))) ==>
+      (VarBind f1 xs ys = VarBind f2 xs ys)``,
+  Induct THEN SIMP_TAC std_ss [VarBind_def,MEM,LIST_TO_SET_THM]
+  THEN1 SRW_TAC [] [DRESTRICT_UNIV] THEN Cases_on `ys`
+  THEN SIMP_TAC std_ss [VarBind_def,MEM,LIST_TO_SET_THM]
+  THEN REPEAT STRIP_TAC THEN Q.PAT_ASSUM `!ys. bbb` MATCH_MP_TAC
+  THEN FULL_SIMP_TAC std_ss [GSYM fmap_EQ_THM,DRESTRICT_DEF,IN_INTER,IN_COMPL,IN_INSERT,EXTENSION,FDOM_FUPDATE,FAPPLY_FUPDATE_THM]
+  THEN METIS_TAC []);
+
+val DRESTRICT_list2fmap = prove(
+  ``!xs ys. DRESTRICT (list2fmap xs) (COMPL (set ys)) =
+            list2fmap (FILTER (\x. ~MEM (FST x) ys) xs)``,
+  Induct THEN SIMP_TAC std_ss [list2fmap_def,FILTER,DRESTRICT_FEMPTY]
+  THEN Cases THEN SIMP_TAC std_ss [list2fmap_def,DRESTRICT_FUPDATE]
+  THEN ASM_SIMP_TAC std_ss [IN_COMPL,IN_LIST_TO_SET]
+  THEN Cases_on `MEM q ys` THEN ASM_SIMP_TAC std_ss [list2fmap_def]);
+
 val R_ev_LEMMA = let
   val th = Q.SPECL [`\(e,a) s. !xs. iR_PERM xs (fmap2list a) ==> iR_ev (e,xs) s`,
                     `\(fn,args,a) s. !xs. iR_PERM xs (fmap2list a) ==> iR_ap (fn,args,xs) s`,
@@ -720,9 +878,13 @@ val R_ev_LEMMA = let
     THEN FULL_SIMP_TAC bool_ss [LIST_LOOKUP_fmap2list_list2fmap]
     THEN MATCH_MP_TAC (el 2 (CONJUNCTS iR_ev_rules))
     THEN ASM_SIMP_TAC std_ss [GSYM FDOM_list2sexp])
-  THEN1 (METIS_TAC [iR_ev_rules])
+  THEN1 (METIS_TAC [iR_ev_rules,iR_ap_LEMMA])
   THEN1
-   (MATCH_MP_TAC (el 8 (CONJUNCTS iR_ev_rules))
+   (MATCH_MP_TAC (el 6 (CONJUNCTS iR_ev_rules)) THEN ASM_SIMP_TAC std_ss [])
+  THEN1
+   (MATCH_MP_TAC (el 8 (CONJUNCTS iR_ev_rules)) THEN ASM_SIMP_TAC std_ss []
+    THEN MATCH_MP_TAC (METIS_PROVE [] ``((c ==> b) /\ c) ==> (b /\ c)``)
+    THEN STRIP_TAC THEN1 METIS_TAC [iR_ap_LEMMA]
     THEN Q.PAT_ASSUM `!xs.bbb` MATCH_MP_TAC
     THEN FULL_SIMP_TAC std_ss [iR_PERM_def,list2fmap_fmap2list]
     THEN ASM_SIMP_TAC std_ss [FunBind_def,iFunBind_def,list2fmap_def])
@@ -733,23 +895,11 @@ val R_ev_LEMMA = let
     THEN FULL_SIMP_TAC bool_ss [LIST_LOOKUP_fmap2list_list2fmap]
     THEN FULL_SIMP_TAC std_ss [FDOM_list2sexp])
   THEN1
-   (FULL_SIMP_TAC std_ss [iR_PERM_EQ]
-    THEN Q.PAT_ASSUM `!s e a. bbb` MATCH_MP_TAC
-    THEN Q.PAT_ASSUM `!xs. bbb` MATCH_MP_TAC
-    THEN FULL_SIMP_TAC std_ss [iR_PERM_def,list2fmap_fmap2list]
-    THEN POP_ASSUM (K ALL_TAC)
-    THEN POP_ASSUM MP_TAC
-    THEN ASM_SIMP_TAC std_ss [iFunBind_def,iVarBind_def,list2fmap_def]
-    THEN Q.SPEC_TAC (`args`,`ys`)
-    THEN Q.SPEC_TAC (`xl`,`zs`)
-    THEN Q.SPEC_TAC (`xs`,`xs`)
-    THEN Induct_on `zs`
-    THEN Cases_on `ys` THEN SIMP_TAC std_ss [LENGTH,DECIDE ``~(SUC n = 0)``]
-    THEN ASM_SIMP_TAC std_ss [iVarBind_def,VarBind_def]
-    THEN REPEAT STRIP_TAC
-    THEN RES_TAC
-    THEN POP_ASSUM (ASSUME_TAC o GSYM)
-    THEN ASM_REWRITE_TAC [list2fmap_def])
+   (MATCH_MP_TAC (el 10 (CONJUNCTS iR_ev_rules)) THEN ASM_SIMP_TAC std_ss []
+    THEN REPEAT STRIP_TAC THEN Q.PAT_ASSUM `!xs. bbb ==> bbbb` MATCH_MP_TAC
+    THEN FULL_SIMP_TAC std_ss [iR_PERM_EQ,list2fmap_iVarBind]
+    THEN MATCH_MP_TAC VarBind_EQ THEN POP_ASSUM MP_TAC
+    THEN ASM_SIMP_TAC std_ss [DRESTRICT_list2fmap])
   THEN METIS_TAC [iR_ev_rules])
   in th end;
 
