examples/machine-code/lisp/lisp_evalScript.sml
@@ -77,11 +77,6 @@ val (thms,_,_) = compile_all ``
     else
       ^STATE)
   /\
- (lisp_less ^STATE =
-    if getVal exp < getVal x
-    then let exp = Sym "t" in ^STATE
-    else let exp = Sym "nil" in ^STATE)
-  /\
  (lisp_symbolp ^STATE =
     if isSym exp
     then let exp = Sym "t" in ^STATE
@@ -127,12 +122,64 @@ val (thms,_,_) = compile_all ``
     else
       ^STATE)
   /\
+ (lisp_find_in_list ^STATE =
+    if ~(isDot y) then let exp = Sym "nil" in ^STATE else
+      let x = CAR y in
+        if exp = x then let exp = Sym "t" in ^STATE else  
+          let y = CDR y in
+            lisp_find_in_list ^STATE)
+  /\
+ (lisp_reduce_alist_aux ^STATE =
+    if (z = Val 0) then ^STATE else
+    if ~isDot alist then ^STATE else
+      let exp = CAR alist in
+      let exp = CAR exp in
+      let y = CAR stack in
+      let (exp,x,y,z,stack,alist,l) = lisp_find_in_list ^STATE in 
+        if exp = Sym "nil" then ^STATE else
+          let z = LISP_SUB z (Val 1) in
+          let alist = CDR alist in
+            lisp_reduce_alist_aux ^STATE) 
+  /\
+ (lisp_reduce_alist ^STATE = 
+    if isDot stack then 
+      let z = CAR stack in
+        if isDot z then ^STATE else
+        if isSym z then ^STATE else
+          let x = CDR stack in
+          let exp = Dot exp x in
+          let x = y in
+          let y = CAR y in
+          let exp = Dot exp x in
+          let x = exp in
+          let exp = y in
+          let exp = Dot exp x in
+          let stack = exp in  
+          let (exp,x,y,z,stack,alist,l) = lisp_reduce_alist_aux ^STATE in
+          let stack = CDR stack in
+          let y = CDR stack in
+          let stack = CAR stack in
+          let exp = CAR stack in 
+          let stack = CDR stack in
+            if z = Val 0 then ^STATE else
+              let x = z in
+              let z = exp in
+              let exp = x in
+              let x = stack in
+              let exp = Dot exp x in
+              let stack = exp in
+              let exp = z in
+                ^STATE
+    else ^STATE)
+  /\
  (lisp_func ^STATE =
     if isDot x then
       let y = CDR x in
       let x = CAR x in
         if x = Sym "lambda" then
-          let z = exp in      (* z := evaluated args   *)
+          let x = CAR y in    
+          let (exp,x,y,z,stack,alist,l) = lisp_reduce_alist ^STATE in
+          let z = exp in      (* z hold evaluated args   *)
           let x = exp in
           let exp = Val 0 in
           let (exp,x,y,z,stack,alist,l) = lisp_length ^STATE in
